Initial work on map iteration

go/iterator/iter_test.go
@@ -49,3 +49,37 @@ func TestReverseSlice0(t *testing.T) {
 		t.Errorf(`[7 ... 0] was not reversed correctly!`)
 	}
 }
+
+func TestMapDeepEqualEmpty(t *testing.T) {
+	if !mapDeepEqual(map[int]int{}, map[int]int{}) {
+		t.Errorf(`Empty maps are not equal!`)
+	}
+}
+
+func TestMapDeepEqualSubmaps(t *testing.T) {
+	fullmap := map[int]int{0: 0, 1: 1, 2: 2}
+	submap := map[int]int{0: 0, 1: 1}
+
+	if mapDeepEqual(fullmap, submap) ||
+		mapDeepEqual(submap, fullmap) {
+		t.Errorf(`Submaps are not equal!`)
+	}
+}
+
+func TestMapDeepEqualIntersect(t *testing.T) {
+	m1 := map[int]int{0 : 0, 1 : 1, 2 : 2}
+	m2 := map[int]int{1 : 1, 2 : 2, 3 : 3}
+
+	if mapDeepEqual(m1, m2) || mapDeepEqual(m2, m1) {
+		t.Errorf(`Intersecting maps are not necessarily equal!`)
+	}
+}
+
+func TestMapDeepEqualTrue(t *testing.T) {
+	m1 := map[int]int{0: 0, 1: 1, 2: 2}
+	m2 := map[int]int{2: 2, 1: 1, 0: 0}
+
+	if !mapDeepEqual(m1, m2) || !mapDeepEqual(m1, m2) {
+		t.Errorf(`Equal maps aren't equal!`)
+	}
+}
