go/iterator/map_iter.go
@@ -1,0 +1,36 @@
+package iterator
+
+func mapIter[K comparable, V comparable](m map[K]V) func(yield func(K, V) bool) {
+	return func(yield func(K, V) bool) {
+		for k, v := range m {
+			if !yield(k, v) {
+				return
+			}
+		}
+	}
+}
+
+func mapDeepEqual[K comparable, V comparable](m1, m2 map[K]V) bool {
+	if len(m1) != len(m2) {
+		return false
+	}
+
+	ret_val := true
+
+	loop_body := func(k1 K, v1 V) bool {
+		v2, present := m2[k1]
+
+		if !present || v1 != v2 {
+			ret_val = false
+			return false
+		}
+
+		return true
+	}
+
+	iterator := mapIter[K, V](m1)
+
+	iterator(loop_body)
+
+	return ret_val
+}
