src/iter/map_iter.v
@@ -1,0 +1,41 @@
+From sys_verif.program_proof Require Import prelude empty_ffi.
+From New.proof Require Import std.
+From New.generatedproof.sys_verif_code Require Import iterator.
+
+Section proof.
+Context `{hG: !heapGS Σ} `{!globalsGS Σ} {go_ctx: GoContext}.
+
+#[global] Instance : IsPkgInit iterator := define_is_pkg_init True%I.
+#[global] Instance : GetIsPkgInitWf iterator := build_get_is_pkg_init_wf.
+
+Definition is_mapIter `{Countable K} `{!IntoVal K} `{!IntoVal V} (mapIter : func.t)
+    (m : gmap K V) (P : gmap K V → iPropI Σ) Φ : iPropI Σ :=
+  ∀ (yield : func.t), (
+    "HP" :: P(∅) ∗
+    "#Hyield" :: □(
+      ∀ (k : K) (v : V) (sm : gmap K V),
+        (⌜ (<[ k := v ]> sm) ⊆ m ⌝ ∗ P(sm)) -∗
+        WP #yield #k #v {{
+          ok,
+          if (decide (ok = #true)) then
+            P(<[ k := v ]> sm)
+          else if (decide (ok = #false)) then
+            Φ
+          else
+            False
+        }}
+    ) ∗
+    "Htrace" :: (P(m) -∗ Φ)
+  )%I -∗
+  WP #mapIter #yield {{ _, Φ }}.
+
+Lemma wp_mapIter `{Countable K} `{!IntoVal K} `{!IntoValTyped K kt} `{!IntoVal V} `{!IntoValTyped V vt} 
+    mref (m : gmap K V) P Φ' :
+  {{{
+    is_pkg_init iterator ∗
+    "#Hmap" :: own_map mref DfracDiscarded m
+  }}}
+    @! iterator.mapIter #kt #vt #mref
+  {{{ (f : func.t), RET #f; is_mapIter f m P Φ' }}}.
+Proof.
+Admitted.
